manually revert IncrementWait to using separate register for status

investigations/bedrock2/IncrementWait/Constants.v
@@ -7,4 +7,9 @@ Definition READ := "MMIOREAD".
 Definition WRITE := "MMIOWRITE".
 
 Definition VALUE_ADDR: Z := 16 * 2^10.
-Definition STATUS_ADDR: Z := 16 * 2^10.
+Definition STATUS_ADDR: Z := 16 * 2^10 + 4.
+
+Definition STATUS_IDLE: Z := 0.
+Definition STATUS_BUSY: Z := 1.
+Definition STATUS_DONE: Z := 2.
+
