investigations/bedrock2/IncrementWait/IncrementWaitSemantics.v
@@ -61,8 +61,15 @@ Section WithParameters.
     | STATUS => word.of_Z STATUS_ADDR
     end.
 
-  Definition status_value (flag : word) : word :=
-    word.slu (word.of_Z 1) flag.
+  Definition status_flag (s : state) : word :=
+    match s with
+    | IDLE => word.of_Z STATUS_IDLE
+    | BUSY _ _ => word.of_Z STATUS_BUSY
+    | DONE _ => word.of_Z STATUS_DONE
+    end.
+
+  Definition status_value (flag : Z) : word :=
+    word.slu (word.of_Z 1) (word.of_Z flag).
 
   (* circuit spec *)
   Definition proc : word -> word := word.add (word.of_Z 1).
@@ -72,14 +79,13 @@ Section WithParameters.
     match r with
     | STATUS =>
       match s with
-      | IDLE => val = word.of_Z 0 /\ s' = IDLE
-      | DONE answer => val = status_value (word.of_Z 31) /\ s' = DONE answer
+      | IDLE => val = status_value STATUS_IDLE /\ s' = IDLE
+      | DONE answer => val = status_value STATUS_DONE /\ s' = DONE answer
       | BUSY input n =>
         (* either the status is DONE and we transition to the DONE state *)
-        (val = status_value (word.of_Z 31) /\ s' = DONE (proc input))
+        (val = status_value STATUS_DONE /\ s' = DONE (proc input))
         (* ...or the status is BUSY and we stay in the BUSY state *)
-        \/ (exists n', n = S n' /\ word.and val (word.sru (word.of_Z 1) (word.of_Z 31)) = word.of_Z 0
-                       /\ s' = BUSY input n')
+        \/ (exists n', n = S n' /\ val = status_value STATUS_BUSY /\ s' = BUSY input n')
       end
     | VALUE =>
       match s with
